Reorderer/Impl.v
@@ -43,7 +43,7 @@ Section Reorderer.
     Section withTy.
       Definition sendReq
                  ty
-                 (isError : immResT @# ty -> Bool @# ty)
+                 (isError : immResK @# ty -> Bool @# ty)
                  (memReq
                   : ty ReordererArbiterReq ->
                     ActionT ty ReordererImmRes)
@@ -88,10 +88,10 @@ Section Reorderer.
           DispString _ "[Reorderer.reordererCallback]\n"
         ];
         LET idx: ReordererReqId <- #resp @% "tag";
-        LET res: mInstT <- #resp @% "resp";
+        LET res: mInstK <- #resp @% "resp";
         Read valids: Array numReqId Bool <- validArray;
         Write validArray: Array numReqId Bool <- #valids@[#idx <- $$true];
-        WriteRf rfWrite(#idx: reqIdSz ; #res: mInstT);
+        WriteRf rfWrite(#idx: reqIdSz ; #res: mInstK);
         System [
           DispString _ "[Reorderer.reordererCallback] stored response:\n";
           DispHex #res;
@@ -113,7 +113,7 @@ Section Reorderer.
            LET deqP: ReordererReqId
                        <- UniBit (TruncLsb _ 1)
                        (castToReqIdSz (fun n => Expr ty (SyntaxKind (Bit (n + 1)))) #deqPFull);
-           ReadRf inst: mInstT <- rfRead(#deqP: ReordererReqId);
+           ReadRf inst: mInstK <- rfRead(#deqP: ReordererReqId);
            ReadRf vaddrInfo: ReordererStorage <- arfRead(#deqP: ReordererReqId);
            LET resp
            :  ReordererRes
@@ -146,7 +146,7 @@ Section Reorderer.
     Definition regFiles: list RegFileBase :=
       [ 
         @Build_RegFileBase false 1 rfName
-                           (Async [rfRead]) rfWrite (Nat.pow 2 reqIdSz) mInstT (@RFNonFile _ _ None);
+                           (Async [rfRead]) rfWrite (Nat.pow 2 reqIdSz) mInstK (@RFNonFile _ _ None);
           
         @Build_RegFileBase false 1 arfName
                            (Async [arfRead]) arfWrite (Nat.pow 2 reqIdSz) ReordererStorage (@RFNonFile _ _ None)
